

Part B

$$x = \begin{bmatrix} 20 \\ 3 \\ 4 \end{bmatrix}, y = 18, b_2 = [0,5]$$

$$w_1 = \begin{bmatrix} 0,2 & 0,2 & 0,3 \\ 0,4 & 0,5 & 0,6 \\ 0,7 & 0,8 & 0,9 \end{bmatrix} \quad b_1 = \begin{bmatrix} 0,1 \\ 0,2 \\ 0,3 \end{bmatrix}$$

$$w_2 = [0,2; 0,4; 0,6]$$

Forward Propagation

$$1. z_1 = w_1 \cdot x + b_1$$

$$z_1 = \begin{bmatrix} 0,2 & 0,2 & 0,3 \\ 0,4 & 0,5 & 0,6 \\ 0,7 & 0,8 & 0,9 \end{bmatrix} \cdot \begin{bmatrix} 20 \\ 3 \\ 4 \end{bmatrix} + \begin{bmatrix} 0,1 \\ 0,2 \\ 0,3 \end{bmatrix}$$

$$R_1 = (0,4 \cdot 20) + (0,2 \cdot 3) + (0,3 \cdot 4) + 0,1 = 3,9$$

$$R_2 = (0,4 \cdot 20) + (0,5 \cdot 3) + (0,6 \cdot 4) + 0,2 = 12,1$$

$$R_3 = (0,7 \cdot 20) + (0,8 \cdot 3) + (0,9 \cdot 4) + 0,3 = 20,3$$

$$z_1 = \begin{bmatrix} 3,9 \\ 12,1 \\ 20,3 \end{bmatrix}$$

$$A_1 = \text{ReLU}(z_1) \text{ where } \text{ReLU}(x) = \max(0, x)$$

$$2. A_1 = \begin{bmatrix} 3,9 \\ 12,1 \\ 20,3 \end{bmatrix} \text{ because all values positive}$$

$$3. z_2 = w_2 \cdot A_1 + b_2$$

$$z_2 = [0,2 \cdot 0,4 \quad 0,6] \cdot \begin{bmatrix} 3,9 \\ 12,1 \\ 20,3 \end{bmatrix} + [0,5]$$

$$z_2 = (0,2 \cdot 3,9) + (0,4 \cdot 12,1) + (0,6 \cdot 20,3) + 0,5 = 18,3$$

$$z_2 = 18,3$$

4. $f_2 = \text{sigmoid}(z_2)$ where $\sigma(x) = 1/(1+e^{-x})$

$$A_2 = \text{sigmoid}(18,3) = \frac{1}{1+e^{-18,3}} \approx 1$$

5. Calculate loss $= (f_2 - y)^2$ where $y = 18$

$$\text{loss} = (1 - 18)^2 = (-18)^2 = 288$$

Backward Propagation

1. $dL/dA_2 = 2(A_2 - y) = 2(1 - 18) \approx -34$

2. $dL/dz_2 = dL/dA_2 \cdot \text{sigmoid}'(z_2)$ where $\text{sigmoid}'(z) = \sigma(z)(1 - \sigma(z))$

$$\text{sigmoid}'(z) = \sigma(z)(1 - \sigma(z))$$

$$dL/dz_2 = -34 \cdot 1,12 \cdot 10^{-8} = -3,8 \cdot 10^{-7}$$

3. $dL/dW_2 = dL/dz_2 \cdot A_1^T = -3,8 \cdot 10^{-7} \cdot [3,9 \ 12,1 \ 20,5] =$
 $= [-1,49 \cdot 10^{-6} \ -4,61 \cdot 10^{-6} \ -7,73 \cdot 10^{-6}]$

4. $dL/dz_2 = dL/dA_2 = -3,8 \cdot 10^{-7}$

5. $dL/dA_1 = W_2^T \cdot dL/dz_2 = \begin{bmatrix} 0,2 \\ 0,4 \\ 0,6 \end{bmatrix} \cdot -3,8 \cdot 10^{-7} =$
 $= \begin{bmatrix} -1,52 \cdot 10^{-8} \\ -1,52 \cdot 10^{-7} \\ -2,28 \cdot 10^{-7} \end{bmatrix}$

6. $dL/dz_1 = dL/dA_1 \cdot \text{Relu}'(z_1)$ where $\text{Relu}(x) = 1$

if $x > 0$ else 0

$$dL/dz_1 = \begin{bmatrix} -1,52 \cdot 10^{-8} \\ -1,52 \cdot 10^{-7} \\ -2,28 \cdot 10^{-7} \end{bmatrix}$$

$$7. dL/dw_1 = dL/dz_1 \cdot x^T$$

$$dL/dw_1 = \begin{bmatrix} -7,62 \cdot 10^{-8} \\ -1,52 \cdot 10^{-4} \\ -2,23 \cdot 10^{-7} \end{bmatrix} \cdot \begin{bmatrix} 20 & 3 & 4 \end{bmatrix}^T$$

$$= \begin{bmatrix} -1,52 \cdot 10^{-6} & -2,28 \cdot 10^{-4} & -3,04 \cdot 10^{-4} \\ -3,09 \cdot 10^{-5} & -4,56 \cdot 10^{-4} & -6,08 \cdot 10^{-4} \\ -4,52 \cdot 10^{-6} & -6,84 \cdot 10^{-7} & -9,12 \cdot 10^{-7} \end{bmatrix}$$

$$8. dL/db_1 = dL/dz_1$$

$$dL/db_1 = \begin{bmatrix} -7,62 \cdot 10^{-8} \\ -1,52 \cdot 10^{-4} \\ -2,23 \cdot 10^{-7} \end{bmatrix}$$